Tetration works on modular aritimetic?

$$\displaystyle  \begin{array}{{>{\displaystyle}l}}
m\ \box{0} =\ S( m)\\
n\ \textcircled{1} \ \left(\textcircled{0} m\right) =\textcircled{0} \left( n\textcircled{1} m\right)\\
n\ \textcircled{2} \ \left(\textcircled{0} m\right) =n( m+1) =nm+n =\left( n\textcircled{2} m\right)\textcircled{1} n\\
_{x} \ \overset{y}{3} \ =\ _{x} \ \overset{_{x} \ \overset{y-1}{3} \ }{2} \ =_{x} \ \overset{_{x} \ \overset{_{x} \ \overset{_{x} \ \overset{_{x} \ \overset{_{x} \ \overset{_{x} \ \overset{_{x} \ \overset{_{x} \ \overset{y-2}{3} \ }{2} \ }{2} \ }{2} \ }{2} \ \ }{2} \ }{2} \ }{2} \ }{2} \ \\
\\
_{x} \ \overset{y+1}{n+1} \ =\ _{x} \ \overset{_{x} \ \overset{y}{n+1} \ }{n} \ \ \\
\\
_{x} \ \overset{y+1}{n+1} \ =\ _{x} \ \overset{_{x} \ \overset{y}{n+1} \ }{n} \ \ \\
n\ \tikz[baseline=(char.base)]{\node[ellipse,draw] (char) {\textcircled{0} k};}
\ \left(\textcircled{0} m\right) =\left( n\tikz[baseline=(char.base)]{\node[ellipse,draw] (char) {\textcircled{0} k};}
m\right)\textcircled{k} n
\end{array}$$



$$\displaystyle n\xrightarrow{F}\left( x\rightarrow \left( y\rightarrow z\right)\right)$$

$$\displaystyle  \begin{array}{{>{\displaystyle}l}}
F( n+1)( x)( y+1) =F( n)( x)( F( n+1)( x)( y))\\
F( n+1)( x)( y) =F( n)( x)( F( n)( x)( F( n)( x)( F( n+1)( x)( y-3))))\\
=( F( n)( x))^{y}( 1)\\
F( n+1)( x)( y) =( F( n)( x))^{-}( F( n+1)( x)( y+1))
\end{array}$$





$$\displaystyle  \begin{array}{{>{\displaystyle}l}}
_{a_{2}}^{b_{2}}[ 1] =a_{2} +b_{2} =c_{2} \Leftrightarrow \\
_{a_{2}}^{b_{2}}[ 2] =a_{2} \cdot b_{2} =c_{2} \ \Leftrightarrow \ a_{2} =^{b_{2}}[ 2]_{c_{2}} =\frac{b_{2}} \Leftrightarrow b_{2} =_{a_{2}}[ 2]_{c_{2}} =a_{2} /c_{2}\\
_{a_{3}}^{b_{3}}[ 3] =a_{3}^{b_{3}} =c_{3} \ \Leftrightarrow \ a_{3} =^{b_{3}}[ 3]_{c_{3}} =\sqrt[b_{3}]{c_{3}} \ \Leftrightarrow b_{3} =_{a_{3}}[ 3]_{c_{3}} =\log_{a_{3}} c_{3}\\
a_{3}^{b_{3} +1} =a_{3} \cdot a_{3}^{b_{3}}\\
_{a_{3}}^{b_{3} +1}[ 2+1] =_{a_{3}}^{_{a_{3}}^{b_{3}}[ 2+1]}[ 2]\\
\\
a=_{b} n_{c} =_{^{a} n_{c}} n_{c} =_{b} n_{_{b}^{a} n} =_{^{a} n_{c}} n_{_{b}^{a} n}\\
b=^{a} n_{c} =^{_{b} n_{c}} n_{c} =^{a} n_{_{b}^{a} n} =^{_{b} n_{c}} n_{_{b}^{a} n}\\
c=_{b}^{a} n=_{b}^{_{b} n_{c}} n=_{^{a} n_{c}}^{a} n=_{^{a} n_{c}}^{_{b} n_{c}} n\\
_{a}[ n+1]_{b+1} =_{a}[ n]_{_{a}[ n+1]_{b}} =\underbrace{_{a} n_{_{a} n_{_{a} n_{_{a} n_{_{a} n_{_{a} n_{_{a} n_{_{a} n_{_{a}( S( n))_{b-7}}}}}}}}}}_{S( b) \ \times }\\
\\
_{a}[ n+1]_{b} =_{a}^{_{a}[ n+1]_{b+1}}[ n] =_{a}^{_{a}^{_{a}^{_{a}^{_{a}[ n+4]_{b+4}}[ n]}[ n]}[ n]}[ n]\\
\\
a=b^{c}\\
\\
a=_{b} n( c) =_{b} n^{c}( 1)\\
b=n_{a}( c)\\
c=_{b} n_{a}
\end{array}$$



Commutative Hyper Operations

$$\displaystyle F_{n+1}( a,b) =\exp( F_{n}(\ln( a) ,\ln( b)) =\overset{F_{n}(_{e} \triangle _{a} \ ,\ _{e} \triangle _{b})}{_{e} \triangle }$$